\documentclass[hidelinks]{ctexart}

\usepackage{van-de-la-illinoise}

\begin{document}

\section{微分算子法} % (fold)
\label{sec:微分算子法}

\begin{ex}
    $\displaystyle \+DtDu = \+D{x^2}D{u}$, $u\pare{x,0} = x^2$.
\end{ex}
\begin{solution}
    $\displaystyle u\pare{x,t_0} = e^{t_0\+DtD{}}u\pare{x}\vert_{t=0} = \brac{1+t\pare{\+D{x^2}D{^2}} + \cdots} x^2 = \boxed{x^2 + 2t.}$
\end{solution}
\begin{ex}
    $\displaystyle \+D{t^2}D{^2 u} = \+D{x^2}D{^2u}$, $u\pare{x,0} = x^2$, $u_t\pare{x,0} = 0$.
\end{ex}
\begin{solution}
    令$\displaystyle v = \+DtDu$, $\displaystyle A = \begin{pmatrix}
        0 & 1 \\
        \displaystyle \+D{x^2}D{^2} & 0
    \end{pmatrix}$, 则
    \begin{align*}
        & \+DtD{}\begin{pmatrix}
            u \\ v
        \end{pmatrix} = \begin{pmatrix}
            0 & 1 \\
            \displaystyle \+D{x^2}D{^2} & 0
        \end{pmatrix}\begin{pmatrix}
            u \\ v
        \end{pmatrix} = A \begin{pmatrix}
            u \\ v
        \end{pmatrix}, \\
        & \begin{pmatrix}
            u \\ v
        \end{pmatrix} = e^{tA}\begin{pmatrix}
            u \\ v
        \end{pmatrix}_{t=0} \\ &= \begin{pmatrix}
            u \\ v
        \end{pmatrix}_{t=0} + t\begin{pmatrix}
            0 & 1 \\
            \displaystyle \+D{x^2}D{^2} & 0
        \end{pmatrix}\begin{pmatrix}
            u \\ v
        \end{pmatrix}_{t=0} + \frac{t^2}{2}\begin{pmatrix}
            \displaystyle \+D{x^2}D{^2} & \\
            & \displaystyle \+D{x^2}D{^2}
        \end{pmatrix}\begin{pmatrix}
            u \\ v
        \end{pmatrix}_{t=0} + \cdots \\
        &= \begin{pmatrix}
            x^2 \\ *
        \end{pmatrix} + t\begin{pmatrix}
            0 \\ *
        \end{pmatrix} + \frac{t^2}{2} \begin{pmatrix}
            2 \\ *
        \end{pmatrix} + \cdots = \boxed{x^2 + t^2.} \qedhere
    \end{align*}
\end{solution}
\begin{ex}
    $\displaystyle \begin{cases}
        \displaystyle \+D{t^2}D{^2u} + 2\+DtDu = \+D{x^2}D{^2u} - u, \quad t>0,\quad -\infty<x<+\infty, \\
        u\pare{0,x} = 0,\quad u_t\pare{0,x} = x.
    \end{cases}$
\end{ex}
\begin{solution}
    记$\displaystyle A = \begin{pmatrix}
        0 & 1 \\
        \partial_{xx}^2 - 1 & -2
    \end{pmatrix}$, 则
    \begin{align*}
        & \+DtD{} \begin{pmatrix}
            u \\ u_t
        \end{pmatrix} = \begin{pmatrix}
        0 & 1 \\
        \partial_{xx}^2 - 1 & -2
    \end{pmatrix}\begin{pmatrix}
        u \\ u_t
    \end{pmatrix} = A \begin{pmatrix}
        u \\ u_t
    \end{pmatrix} \\
        &\Rightarrow\begin{pmatrix}
            u \\ u_t
        \end{pmatrix} = e^{tA}\left.\begin{pmatrix}
        u \\ u_t
    \end{pmatrix}\right\vert_{t=0}
        = e^{tA}\begin{pmatrix}
            0 \\ x
        \end{pmatrix}\\ 
        &= \exp \brac{t \begin{pmatrix}
            & 1 \\
            \partial_{xx}^2 - 1 & -2
        \end{pmatrix}} \begin{pmatrix}
            0 \\ x
        \end{pmatrix} = \exp \brac{t \begin{pmatrix}
            & 1 \\
            - 1 & -2
        \end{pmatrix}} \begin{pmatrix}
            0 \\ x
        \end{pmatrix} \\
        &= \exp \brac{t \begin{pmatrix}
            -1 & 1 \\
            0 & -1
        \end{pmatrix}\begin{pmatrix}
            -1 & 1 \\
            0 & -1
        \end{pmatrix}\begin{pmatrix}
            -1 & 1 \\
            0 & -1
        \end{pmatrix}^{-1}} \begin{pmatrix}
            0 \\ x
        \end{pmatrix} \\
        &= \begin{pmatrix}
            -1 & 1 \\
            0 & -1
        \end{pmatrix}\exp \brac{t \begin{pmatrix}
            -1 & 1 \\
            0 & -1
        \end{pmatrix}}\begin{pmatrix}
            -1 & 1 \\
            0 & -1
        \end{pmatrix}^{-1} \begin{pmatrix}
            0 \\ x
        \end{pmatrix} \\
        &= \begin{pmatrix}
            -1 & 1 \\
            0 & -1
        \end{pmatrix}\begin{pmatrix}
            1 - t + t^2/2! - t^3/3! + \cdot & t - 2t^2/2! + 3t^3/3! - \cdot \\
            & 1 - t + t^2/2! - t^3/3!
        \end{pmatrix}\begin{pmatrix}
            -1 & 1 \\
            0 & -1
        \end{pmatrix}^{-1} \begin{pmatrix}
            0 \\ x
        \end{pmatrix} \\
        &= \begin{pmatrix}
            -1 & 1 \\
            0 & -1
        \end{pmatrix}\begin{pmatrix}
            e^{-t} & te^{-t} \\
            & te^{-t}
        \end{pmatrix}\begin{pmatrix}
            -1 & 1 \\
            0 & -1
        \end{pmatrix}^{-1} \begin{pmatrix}
            0 \\ x
        \end{pmatrix} \\
        &= \begin{pmatrix}
            xte^{-t} \\
            *
        \end{pmatrix}\\
        & \Rightarrow \boxed{u = xte^{-t}.} \qedhere
    \end{align*}
\end{solution}

% section 微分算子法 (end)

\end{document}
