\documentclass[hidelinks]{ctexart}

\usepackage{van-de-la-illinoise}
\usepackage[paper=b5paper,top=.3in,left=.9in,right=.9in,bottom=.3in]{geometry}
\usepackage{calc}
\pagenumbering{gobble}
\setlength{\parindent}{0pt}
\sisetup{inter-unit-product=\ensuremath{{}\cdot{}}}
\usepackage{van-le-trompe-loeil}

\usepackage{stackengine}
\stackMath
\usepackage{scalerel}
\usepackage[outline]{contour}

\newdimen\indexlen
\def\newprobheader#1{%
\def\probindex{#1}
\setlength\indexlen{\widthof{\textbf{\probindex}}}
\hskip\dimexpr-\indexlen-1em\relax
\textbf{\probindex}\hskip1em\relax
}
\def\newprob#1{%
\newprobheader{#1}%
\def\newprob##1{%
\probsep%
\newprobheader{##1}%
}%
}
\def\probsep{\vskip1em\relax{\color{gray}\dotfill}\vskip1em\relax}

\newlength\thisletterwidth
\newlength\gletterwidth
\newcommand{\leftrightharpoonup}[1]{%
{\ooalign{$\scriptstyle\leftharpoonup$\cr%\kern\dimexpr\thisletterwidth-\gletterwidth\relax
$\scriptstyle\rightharpoonup$\cr}}\relax%
}
\def\tensor#1{\settowidth\thisletterwidth{$\mathbf{#1}$}\settowidth\gletterwidth{$\mathbf{g}$}\stackon[-0.1ex]{\mathbf{#1}}{\boldsymbol{\leftrightharpoonup{#1}}}  }
\def\onedot{$\mathsurround0pt\ldotp$}
\def\cddot{% two dots stacked vertically
  \mathbin{\vcenter{\baselineskip.67ex
    \hbox{\onedot}\hbox{\onedot}}%
}}%

\begin{document}

\newprob{4.2 (2)}%
对$t$做Laplace变换后
\[ p^2 \hat u - pu\vert_{t=0} - u'\vert_{t=0} = p^2\hat u - b = a^2 \+D{x^2}D{^2\hat u}. \]
结合自然边界条件得到
\[ \hat u = \frac{b}{p^2}\pare{1-e^{-px/a}}. \]
逆变换为
\[ u = \boxed{bt - H\pare{t-\frac{x}{a}}b\pare{t-\frac{x}{a}}.} \]
\newprob{4.2 (4)}%
对$t$做Laplace变换后
\[ p^2 \hat u - pu\vert_{t=0} - u'\vert_{t=0} = p^2\hat u = a^2 \+D{x^2}D{^2 \hat u} + \frac{p}{p^2+\omega^2}. \]
结合自然边界条件得到
\[ \hat u = \rec{p\pare{p^2+\omega^2}}\pare{1-e^{-px/a}} = \pare{\rec{\omega^2}\rec{p} - \rec{\omega^2}\frac{p}{p^2+\omega^2}}\pare{1-e^{-px/a}}. \]
逆变换为
\begin{align*}
    u &= \rec{\omega^2} - \rec{\omega^2}\cos\pare{\omega t} - H\pare{t-\frac{x}{a}}\brac{\rec{\omega^2} - \rec{\omega^2}\cos \omega\pare{t - \frac{x}{a}}} \\
    &= \boxed{\frac{2}{\omega^2}\sin^2 \frac{\omega t}{2} - H\pare{t-\frac{x}{a}}\frac{2}{\omega^2}\sin^2 \brac{\frac{\omega}{2}\pare{t-\frac{x}{a}}}.}
\end{align*}
\newprob{5.1 (1)}%
$\delta\pare{x} \cos x + \delta\pare{x}\sin x = \delta\pare{x} \cos 0 + \delta\pare{x}\sin 0 = \delta\pare{x}.$
\par
\newprobheader{(2)}%
$\displaystyle \int_{-\infty}^\infty f\pare{x} x\delta'\pare{x} = f\pare{x}x\delta\pare{x}\Big\vert_{-\infty}^\infty - \int_{-\infty}^\infty \pare{f'\pare{x}x + f\pare{x}}\delta\pare{x}\,\rd{x} = -f\pare{0}.$
\par
\newprobheader{(3)}%
$\displaystyle \delta\pare{x} = \delta\pare{-x}$两侧求导即$\delta'\pare{x} = -\delta'\pare{-x}$.
\newprob{5.2}%
$\displaystyle f\pare{x_0,y_0} = \int f\pare{x,y}\delta\pare{x-x_0,y-y_0}\,\rd{x}\,\rd{y}$\\
$\displaystyle = \int f\pare{x,y}\delta\pare{x-x_0,y-y_0}\abs{J}\,\rd{\xi}\,\rd{\eta}$ \\
$\displaystyle = f\pare{\xi_0,\eta_0} = \int f\pare{\xi,\eta}\delta\pare{\xi-\xi_0,\eta-\eta_0}\,\rd{\xi}\,\rd{\eta}$\\
$\displaystyle \Rightarrow \delta\pare{x-x_0,y-y_0} \abs{J} = \delta\pare{\xi-\xi_0,\eta-\eta_0}.$\\
极坐标下$\abs{J} = r$, 故\\
$\displaystyle \delta\pare{x-x_0,y-y_0} = \rec{r}\delta\pare{r-r_0,\theta-\theta_0}.$

\end{document}
