\documentclass[hidelinks]{ctexart}

\usepackage{van-de-la-illinoise}
\usepackage[paper=b5paper,top=.3in,left=.9in,right=.9in,bottom=.3in]{geometry}
\usepackage{calc}
\pagenumbering{gobble}
\setlength{\parindent}{0pt}
\sisetup{inter-unit-product=\ensuremath{{}\cdot{}}}
\usepackage{van-le-trompe-loeil}

\usepackage{stackengine}
\stackMath
\usepackage{scalerel}
\usepackage[outline]{contour}

\newdimen\indexlen
\def\newprobheader#1{%
\def\probindex{#1}
\setlength\indexlen{\widthof{\textbf{\probindex}}}
\hskip\dimexpr-\indexlen-1em\relax
\textbf{\probindex}\hskip1em\relax
}
\def\newprob#1{%
\newprobheader{#1}%
\def\newprob##1{%
\probsep%
\newprobheader{##1}%
}%
}
\def\probsep{\vskip1em\relax{\color{gray}\dotfill}\vskip1em\relax}

\newlength\thisletterwidth
\newlength\gletterwidth
\newcommand{\leftrightharpoonup}[1]{%
{\ooalign{$\scriptstyle\leftharpoonup$\cr%\kern\dimexpr\thisletterwidth-\gletterwidth\relax
$\scriptstyle\rightharpoonup$\cr}}\relax%
}
\def\tensor#1{\settowidth\thisletterwidth{$\mathbf{#1}$}\settowidth\gletterwidth{$\mathbf{g}$}\stackon[-0.1ex]{\mathbf{#1}}{\boldsymbol{\leftrightharpoonup{#1}}}  }
\def\onedot{$\mathsurround0pt\ldotp$}
\def\cddot{% two dots stacked vertically
  \mathbin{\vcenter{\baselineskip.67ex
    \hbox{\onedot}\hbox{\onedot}}%
}}%

\begin{document}

\newprob{1.1(1)}%
$\displaystyle x\+DxDu - y\+DyDu = xyf'\pare{xy} - yxf'\pare{xy} = 0$.
\par
\newprobheader{(2)}%
$\displaystyle \lambda_1\lambda_2 \frac{\partial^2 u}{\partial x^2} - \pare{\lambda_1 + \lambda_2} \frac{\partial^2 u}{\partial x \partial y} + \frac{\partial^2 u}{\partial y^2}$\\
$\displaystyle = \lambda_1\lambda_2 \pare{F'' + G''} - \pare{\lambda_1 + \lambda_2}\pare{\lambda_1 F'' + \lambda_2 G''} + \lambda_1^2 F'' + \lambda_2^2 G'' = 0$.
\par
\newprobheader{(3)}%
$\displaystyle \+DxDu = \frac{e^{-\frac{x^2}{4a^2 t}}}{2a\sqrt{\pi t}} \pare{-\frac{x}{2a^2t}}$,\\
$\displaystyle \frac{\partial^2u}{\partial x^2} = -\frac{e^{-\frac{x^2}{4a^2t}}}{4a^3\sqrt{\pi}t^{3/2}} + \frac{e^{-\frac{x^2}{4a^2 t}}}{2a\sqrt{\pi t}}\cdot \frac{x^2}{4a^4t^2}$. \\
$\displaystyle \+DtDu = -\frac{e^{-\frac{x^2}{4a^2t}}}{4a\sqrt{\pi}t^{3/2}} + \frac{e^{-\frac{x^2}{4a^2 t}}}{2a\sqrt{\pi t}}\cdot \frac{x^2}{4a^2t^2}$.\\
$\displaystyle \Rightarrow \+DtDu=a^2\frac{\partial^2u}{\partial x^2}$.\\
$\displaystyle \lim_{t\rightarrow 0} u\pare{t,x} = \lim_{t\rightarrow 0} \frac{e^{-\frac{x^2}{4a^2t}}}{2a\sqrt{\pi t}} \xlongequal{s=1/t} \lim_{s\rightarrow \infty} \frac{\sqrt{s}e^{-\frac{x^2s}{4a}}}{2a\sqrt{\pi}} = 0,\quad x\neq 0$.

\newprob{1.5}%
\vspace{-\baselineskip}
\begin{wrapfigure}{r}{3cm}%
        \centering%
        \incfig{3cm}{StringTense}%
\end{wrapfigure}%
设绳具有线密度$\rho$, 则略去小量有
\begin{align*}
    \rho \frac{\partial^2 u}{\partial t^2} \,\rd{x} &= \brac{\+vT\pare{x+\rd{x}} - \+vT\pare{x}}\cdot \+uu \\
    &\approx T\pare{x+\rd{x}}\+DxD{u\pare{x+\rd{x}}} - T\pare{x}\+DxD{u\pare{x}} \\
    \Rightarrow \rho \frac{\partial^2 u}{\partial t^2} &= \+DxD{}\brac{T\pare{x}\+DxDu}.
\end{align*}
$T$和下段绳的重力近似相等, $T \approx \rho g\pare{l-x}$,
\[ \Rightarrow \boxed{\rho \frac{\partial^2 u}{\partial t^2} = g\+DxD{}\brac{\pare{l-x}\+DxDu}.} \]

\newprob{1.9}%
$\displaystyle c\rho \+DtD{u\pare{r,t}} = k\laplacian u\pare{r,t} = \frac{k}{r^2}\+DrD{}\pare{r^2\+DrD{u\pare{r,t}}},\quad r<R$.\\
$\displaystyle \brac{hu\pare{r,t} + k\+DrD{u\pare{r,t}}}_{r=R} = h\theta\pare{t}$.\\
$\displaystyle u\pare{r,0} = \varphi\pare{r},\quad r<R$.

\end{document}
